wip

theories/sessiontypes.v
@@ -9,16 +9,16 @@ safe : obj → option tid
 safe w = Some t → blocked t ≠ Some w
 blocked t = None → reducible (es !! i) *)
 
-From iris.proofmode Require Import tactics.
+From iris.proofmode Require Import base tactics classes.
 
 Definition loc := nat.
 
 (*
 We have a heap of channel buffers indexed by loc's (e.g. natural numbers).
-We represent a channel as a pair of buffers.
+We represent a channel as a natural number and a boolean for the polarity of the endpoint
 Each party will put its messages in one buffer and read from the other
 *)
-Definition chan := (loc * loc)%type.
+Definition chan := (loc * bool)%type.
 
 (*
 We have a lambda calculus-based language with natural numbers, closures, and unit.
@@ -45,7 +45,7 @@ with expr :=
     | Fork : expr -> expr
     | Close : expr -> expr.
 
-Definition heap := gmap loc (list val).
+Definition heap := list (list val * list val).
 
 Inductive type :=
     | UnitT : type
@@ -59,7 +59,7 @@ with chan_type :=
     | RecvT : type -> chan_type -> chan_type
     | EndT : chan_type.
 
-Definition envT := list (string * type).
+Notation envT := (gmap string type).
 
 Fixpoint dual ct :=
     match ct with
@@ -70,7 +70,8 @@ Fixpoint dual ct :=
 
 Definition heapT := gmap chan chan_type.
 
-Definition disj_union (a b c : heapT) := a ##ₘ b ∧ c = a ∪ b.
+Definition disj_union {A B : Type} `{EqDecision A, Countable A}
+  (a b c : gmap A B) := b ##ₘ c ∧ a = b ∪ c.
 
 Inductive val_typed : heapT -> val -> type -> Prop :=
     | Unit_typed :
@@ -83,7 +84,7 @@ Inductive val_typed : heapT -> val -> type -> Prop :=
         val_typed Σ2 b bT ->
         val_typed Σ (Pair a b) (PairT aT bT)
     | Fun_typed : ∀ Σ x e a b,
-        typed Σ [(x,a)] e b ->
+        typed Σ {[ x := a ]} e b ->
         val_typed Σ (Fun x e) (FunT a b)
     | Chan_typed : ∀ c ct,
         val_typed {[ c := ct ]} (Chan c) (ChanT ct)
@@ -91,64 +92,52 @@ Inductive val_typed : heapT -> val -> type -> Prop :=
 with typed : heapT -> envT -> expr -> type -> Prop :=
     | Val_typed : ∀ Σ v t,
         val_typed Σ v t ->
-        typed Σ [] (Val v) t
+        typed Σ ∅ (Val v) t
     | Var_typed : ∀ x t,
-        typed ∅ [(x,t)] (Var x) t
+        typed ∅ {[ x := t ]} (Var x) t
     | App_typed : ∀ Σ Σ1 Σ2 Γ Γ1 Γ2 e1 e2 t1 t2,
         disj_union Σ Σ1 Σ2 ->
-        Γ ≡ₚ Γ1 ++ Γ2 ->
+        disj_union Γ Γ1 Γ2 ->
         typed Σ1 Γ1 e1 (FunT t1 t2) ->
         typed Σ2 Γ2 e2 t1 ->
         typed Σ Γ (App e1 e2) t2
-    | Lam_typed : ∀ Σ Γ x e t1 t2,
-        (* TODO: freshness condition: x not in Γ depending on whether Γ_x is Drop
-            Same condition in Let -> factor freshness predicate is_fresh Γ x
-            x not in Γ : is_fresh Γ x
-            Γ_x is Drop : is_fresh Γ x
-            is_fresh Γ x := match Γ !! x with Some t => is_drop t | None => True end.
-            is_fresh Γ x := from_option is_drop True (Γ !! x)
-            Change envT to be a map.
-        *)
-        typed Σ ((x,t1)::Γ) e t2 ->
+    | Lam_typed : ∀ Σ Γ Γ' x e t1 t2,
+        disj_union Γ' Γ {[ x := t1 ]} ->
+        typed Σ Γ' e t2 ->
         typed Σ Γ (Lam x e) (FunT t1 t2)
     | Send_typed : ∀ Σ Σ1 Σ2 Γ Γ1 Γ2 e1 e2 t r,
         disj_union Σ Σ1 Σ2 ->
-        Γ ≡ₚ Γ1 ++ Γ2 ->
-        typed Σ1 Γ e1 (ChanT (SendT t r)) ->
-        typed Σ2 Γ e2 t ->
+        disj_union Γ Γ1 Γ2 ->
+        typed Σ1 Γ1 e1 (ChanT (SendT t r)) ->
+        typed Σ2 Γ2 e2 t ->
         typed Σ Γ (Send e1 e2) (ChanT r)
     | Recv_typed : ∀ Σ Γ e t r,
         typed Σ Γ e (ChanT (RecvT t r)) ->
         typed Σ Γ (Recv e) (PairT t (ChanT r))
-    | Let_typed : ∀ Σ Σ1 Σ2 Γ Γ1 Γ2 e1 e2 t1 t2 x,
+    | Let_typed : ∀ Σ Σ1 Σ2 Γ Γ1 Γ2 Γ2' e1 e2 t1 t2 x,
         disj_union Σ Σ1 Σ2 ->
-        Γ ≡ₚ Γ1 ++ Γ2 ->
+        disj_union Γ Γ1 Γ2 ->
+        disj_union Γ2' Γ2 {[ x := t1 ]} ->
         typed Σ1 Γ1 e1 t1 ->
-        typed Σ2 ((x,t1)::Γ2) e2 t2 ->
+        typed Σ2 Γ2' e2 t2 ->
         typed Σ Γ (Let x e1 e2) t2
     | LetUnit_typed : ∀ Σ Σ1 Σ2 Γ Γ1 Γ2 e1 e2 t,
         disj_union Σ Σ1 Σ2 ->
-        Γ ≡ₚ Γ1 ++ Γ2 ->
+        disj_union Γ Γ1 Γ2 ->
         typed Σ1 Γ1 e1 UnitT ->
         typed Σ2 Γ2 e2 t ->
         typed Σ Γ (LetUnit e1 e2) t
-    | LetProd_typed : ∀ Σ Σ1 Σ2 Γ Γ1 Γ2 e1 e2 t11 t12 t2 x1 x2,
+    | LetProd_typed : ∀ Σ Σ1 Σ2 Γ Γ1 Γ2 Γ2' e1 e2 t11 t12 t2 x1 x2,
         disj_union Σ Σ1 Σ2 ->
-        Γ ≡ₚ Γ1 ++ Γ2 ->
+        disj_union Γ Γ1 Γ2 ->
+        x1 ≠ x2 ->
+        disj_union Γ2' Γ2 (<[ x1 := t11 ]> {[ x2 := t12 ]}) ->
         typed Σ1 Γ1 e1 (PairT t11 t12) ->
-        typed Σ2 ((x1,t11)::(x2,t12)::Γ2) e2 t2 ->
+        typed Σ2 Γ2' e2 t2 ->
         typed Σ Γ (LetProd x1 x2 e1 e2) t2
-    (* TODO: LetProd & LetUnit *)
-    (* TODO: Shadowing
-    0. Freshness condition depending on whether the type is Drop
-    1. Barendreght convention, subst renames
-    2. De Bruijn -> no shadowing, but environments more complicated (with options, or maps)
-    3. Explicit environments in op sem -> Hoare logic mismatch
-    4. Subst as a constructor of expr
-    *)
     | If_typed : ∀ Σ Σ1 Σ2 Γ Γ1 Γ2 e1 e2 e3 t,
-        Γ ≡ₚ Γ1 ++ Γ2 ->
         disj_union Σ Σ1 Σ2 ->
+        disj_union Γ Γ1 Γ2 ->
         typed Σ1 Γ1 e1 NatT ->
         typed Σ2 Γ2 e2 t ->
         typed Σ2 Γ2 e3 t ->
@@ -160,44 +149,79 @@ with typed : heapT -> envT -> expr -> type -> Prop :=
         typed Σ Γ e (ChanT EndT) ->
         typed Σ Γ (Close e) UnitT.
 
-(* FIXME: implement substitution *)
-Definition subst (x:string) (a:val) (e:expr) : expr := Val Unit.
+Fixpoint subst (x:string) (a:val) (e:expr) : expr :=
+  match e with
+  | Val _ => e
+  | Var x' => if decide (x = x') then Val a else e
+  | App e1 e2 => App (subst x a e1) (subst x a e2)
+  | Lam x' e1 => if decide (x = x') then e else Lam x' (subst x a e1)
+  | Send e1 e2 => Send (subst x a e1) (subst x a e2)
+  | Recv e1 => Recv (subst x a e1)
+  | Let x' e1 e2 => Let x' (subst x a e1) (if decide (x = x') then e2 else subst x a e2)
+  | LetUnit x' e1 => LetUnit x' (subst x a e1)
+  | LetProd x' y' e1 e2 =>
+      LetProd x' y' (subst x a e1) (if decide (x = x' ∨ x = y') then e2 else subst x a e2)
+  | If e1 e2 e3 => If (subst x a e1) (subst x a e2) (subst x a e3)
+  | Fork e1 => Fork (subst x a e1)
+  | Close e1 => Close (subst x a e1)
+  end.
+
+Definition lookup_recv (h : heap) (c : chan) : option (list val) :=
+  h !! c.1 ≫= λ '(x,y), Some (if c.2 then x else y).
+
+Definition lookup_send (h : heap) (c : chan) : option (list val) :=
+  h !! c.1 ≫= λ '(x,y), Some (if c.2 then y else x).
+
+Definition set_recv (h : heap) (c : chan) (buf : list val) : heap :=
+  let (l,b) := c in
+  match h !! l with
+  | Some (x,y) => <[ l := if b then (buf,y) else (x,buf) ]> h
+  | None => h
+  end.
+Definition set_send (h : heap) (c : chan) (buf : list val) : heap :=
+  let (l,b) := c in
+  match h !! l with
+  | Some (x,y) => <[ l := if b then (x,buf) else (buf,y) ]> h
+  | None => h
+  end.
 
 Inductive head_step : expr -> heap -> expr -> heap -> Prop :=
-    | App_head_step : ∀ x e s a,
-        head_step (App (Val (Fun x e)) (Val a)) s (subst x a e) s
-    | Lam_head_step : ∀ x e s,
-        head_step (Lam x e) s (Val (Fun x e)) s
-    | Send_head_step : ∀ s l1 l2 y buf,
-        s !! l1 = Some buf ->
-        head_step (Send (Val (Chan (l1,l2))) (Val y)) s (Val (Chan (l1,l2))) (<[l1 := y::buf]> s)
-    | Recv_head_step : ∀ s l1 l2 y buf,
-        s !! l2 = Some (y :: buf) ->
-        head_step (Recv (Val (Chan (l1,l2)))) s (Val (Pair (Chan (l1,l2)) y)) (<[l2 := buf]> s)
-    | If_head_step1 : ∀ n s e1 e2,
+    | App_head_step : ∀ x e h a,
+        head_step (App (Val (Fun x e)) (Val a)) h (subst x a e) h
+    | Lam_head_step : ∀ x e h,
+        head_step (Lam x e) h (Val (Fun x e)) h
+    | Send_head_step : ∀ h c y buf,
+        lookup_send h c = Some buf ->
+        head_step (Send (Val (Chan c)) (Val y)) h (Val (Chan c)) (set_recv h c (buf ++ [y]))
+    | Recv_head_step : ∀ h c y buf,
+        lookup_recv h c = Some (y::buf) ->
+        head_step (Recv (Val (Chan c))) h (Val (Pair (Chan c) y)) (set_send h c buf)
+    | If_head_step1 : ∀ n h e1 e2,
         n ≠ 0 ->
-        head_step (If (Val (Nat n)) e1 e2) s e1 s
-    | If_head_step2 : ∀ s e1 e2,
-        head_step (If (Val (Nat 0)) e1 e2) s e2 s
-    | Let_head_step : ∀ x v e s,
-        head_step (Let x (Val v) e) s (subst x v e) s
-    | LetUnit_head_step : ∀ e s,
-        head_step (LetUnit (Val Unit) e) s e s
-    | LetProd_head_step : ∀ x1 x2 v1 v2 e s,
-        head_step (LetProd x1 x2 (Val (Pair v1 v2)) e) s (subst x1 v1 $ subst x2 v2 e) s
-    | Close_step : ∀ l1 l2 s,
-        head_step (Close (Val (Chan (l1,l2)))) s (Val Unit) (delete l2 s).
+        head_step (If (Val (Nat n)) e1 e2) h e1 h
+    | If_head_step2 : ∀ h e1 e2,
+        head_step (If (Val (Nat 0)) e1 e2) h e2 h
+    | Let_head_step : ∀ x v e h,
+        head_step (Let x (Val v) e) h (subst x v e) h
+    | LetUnit_head_step : ∀ e h,
+        head_step (LetUnit (Val Unit) e) h e h
+    | LetProd_head_step : ∀ x1 x2 v1 v2 e h,
+        head_step (LetProd x1 x2 (Val (Pair v1 v2)) e) h (subst x1 v1 $ subst x2 v2 e) h
+    | Close_step : ∀ c h,
+        lookup_recv h c = Some [] ->
+        head_step (Close (Val (Chan c))) h (Val Unit) h.
 
 Lemma head_step_deterministic e s e1 e2 s1 s2 :
     head_step e s e1 s1 -> head_step e s e2 s2 -> e1 = e2 ∧ s1 = s2.
 Proof.
     intros H1 H2.
     induction H1; inversion H2; auto.
-    - rewrite H in H7. simplify_eq. auto.
+Admitted.
+    (* - rewrite H in H7. simplify_eq. auto.
     - rewrite H in H6. simplify_eq. auto.
     - simplify_eq.
     - simplify_eq.
-Qed.
+Qed. *)
 
 Inductive ctx1 : (expr -> expr) -> Prop :=
     | Ctx_App_l : ∀ e, ctx1 (λ x, App x e)
@@ -259,7 +283,7 @@ Proof.
 Qed.
 
 Inductive ctx_step : expr -> heap -> expr -> heap -> Prop :=
-    | Ctx_step : ∀ k e1 e2 s1 s2, 
+    | Ctx_step : ∀ k e1 e2 s1 s2,
         ctx k -> head_step e1 s1 e2 s2 -> ctx_step (k e1) s1 (k e2) s2.
 
 Lemma ctx_step_deterministic e s e1 e2 s1 s2 :
@@ -270,6 +294,7 @@ Proof.
     assert (e3 = e5 ∧ s1 = s2) as (-> & ->) by (eapply head_step_deterministic; eauto); eauto.
 Qed.
 
+(* TODO: make this a relation on pairs, then steps = rtc step *)
 (* We put the fork step here because it needs to spawn a new thread. *)
 Inductive step : list expr -> heap -> list expr -> heap -> Prop :=
     | Head_step : ∀ e1 e2 s1 s2 es i k,
@@ -277,17 +302,15 @@ Inductive step : list expr -> heap -> list expr -> heap -> Prop :=
         head_step e1 s1 e2 s2 ->
         es !! i = Some (k e1) ->
         step es s1 (<[i := (k e2)]> es) s2
-    | Fork_step : ∀ (es : list expr) i v (s : heap) (l1 l2 : loc) k,
+    | Fork_step : ∀ (es : list expr) i v (h : heap) k,
+        let l := length h in
         ctx k ->
         es !! i = Some (k $ Fork (Val v)) ->
-        s !! l1 = None ->
-        s !! l2 = None ->
-        l1 ≠ l2 ->
-        step es s
-            (<[i := k $ Val (Chan (l2,l1))]> es ++ [App (Val v) (Val (Chan (l1,l2)))])
-            (<[l1 := []]> $ <[l2 := []]> s).
+        step es h
+            (<[i := k $ Val (Chan (l,true))]> es ++ [App (Val v) (Val (Chan (l,false)))])
+            (h++[([],[])]).
 
-(* Closure of the step relation; this is used in the theorem heapment. *)
+(* Closure of the step relation; this is used in the theorem statement. *)
 Inductive steps : list expr -> heap -> list expr -> heap -> Prop :=
     | Trans_step : ∀ e1 e2 e3 s1 s2 s3,
         step e1 s1 e2 s2 ->
@@ -299,93 +322,414 @@ Inductive steps : list expr -> heap -> list expr -> heap -> Prop :=
 Inductive all_values : list expr -> Prop :=
     | AV_nil : all_values []
     | AV_cons : ∀ es v, all_values es -> all_values (Val v :: es).
+    (* TODO: add case for waiting on Recv on an empty buffer for now *)
 
-(* TODO: make into big disjoint union predicate *)
 Definition disjoint (xs : list heapT) :=
     forall i j h1 h2, i ≠ j ->
         xs !! i = Some h1 -> xs !! j = Some h2 -> h1 ##ₘ h2.
 
-Definition connected (hs : list heapT) (i j : nat) :=
+Fixpoint disjoint_union {A B : Type} `{Countable A}
+                        (x : gmap A B) (ys : list (gmap A B)) :=
+    match ys with
+    | [] => x = ∅
+    | y::ys' => ∃ x', disj_union x x' y ∧ disjoint_union x' ys'
+    end.
+
+(* Definition connected (hs : list heapT) (i j : nat) :=
     ∃ h1 h2 (l1 l2 : loc) (t : chan_type),
         hs !! i = Some h1 ∧ hs !! j = Some h2 ∧
         h1 !! (l1,l2) = Some t ∧ h2 !! (l2,l1) = Some (dual t).
-        (* TODO: the things in the buffers *)
+        (* TODO: how to handle the things in the buffers?? *)
 
-Inductive is_undirected_tree (T : nat -> nat -> Prop) : Prop := .
+Definition unidirect (T : nat -> nat -> Prop) i j := i < j ∧ T i j.
 
-Definition invariant (es : list expr) (s : heap) : Prop :=
-(*
-    This invariant should make sure that either all es are values or some e in es can take a step.
-    We need to ensure that the expr and heap are well typed.
-    And we need to ensure that we have an acyclic connectivity graph.
-    Picture the current heap as a graph with threads as vertices.
-    The vertices are connected by channels, so each edge stores a channel.
-    A channel consists of a pair of buffers and a channel type for each endpoint.
-    The channel types are dual up to what is already stored in the buffer.
-    The connectivity graph must be acyclic.
-*)
-    ∃ Σs, Forall2 (λ Σ e, typed Σ [] e UnitT) Σs es ∧
-        disjoint Σs ∧ is_undirected_tree (connected Σs).
-    (* disjoint_union Σs Σ ∧ heap_typed Σ s *)
-(*
-PLAN:
-1. naming/shadowing
-2. safety, invariant
-    ask Stephanie: TAPL for session types?
-3. deadlocks
-*)
-    (*
-    Q: What about the elements already in the buffer?
-       This can mean that one session type is ahead of the other.
-    Q: What about channels that sit in a buffer?
-    *)
-    (* TODO: figure out invariant
-        * Maintain graph + acyclicity predicate
-        * Or maintain Coq tree with tree rotations/surgery
-     *)
+Definition is_undirected_tree (T : nat -> nat -> Prop) : Prop :=
+  Symmetric T ∧ Irreflexive (tc (unidirect T)). *)
 
-Theorem invariant_init e : invariant [e] ∅.
-Admitted.
 
-Theorem invariant_step e1 s1 e2 s2 :
-    invariant e1 s1 ->
-    step e1 s1 e2 s2 ->
-    invariant e2 s2.
-Admitted.
-(*
-    For steps not involving channels, we need to ensure that they preserve types.
-    The interesting steps are fork, send, recv.
+Inductive bufs_typed : heapT * list val * chan_type -> heapT * list val * chan_type -> Prop :=
+  | BT_emp : ∀ ct, bufs_typed (∅, [], ct) (∅, [], dual ct)
+  | BT_consL : ∀ Σ Σ1 Σ2 v vT vs ct c,
+    disj_union Σ Σ1 Σ2 ->
+    val_typed Σ1 v vT ->
+    bufs_typed (Σ2, vs, ct) (∅, [], c) ->
+    bufs_typed (Σ, v::vs, ct) (∅, [], RecvT vT c)
+  | BT_consR : ∀ Σ Σ1 Σ2 v vT vs ct c,
+    disj_union Σ Σ1 Σ2 ->
+    val_typed Σ1 v vT ->
+    bufs_typed (∅, [], c) (Σ2, vs, ct) ->
+    bufs_typed (∅, [], RecvT vT c) (Σ, v::vs, ct).
 
-    Fork creates a new thread in the connectivity graph. The parent thread gives some of its linear resources to
-    the forked thread. Finally, we insert an edge between the forked thread and the parent thread, which has a
-    channel with dual session types and empty buffers. So this preserves the invariant.
+Definition invariant (es : list expr) (h : heap) : Prop :=
+  ∃ (Σ : heapT) (Σs : list heapT) (Σh1 Σh2 : list heapT),
+    disjoint_union Σ (Σh1 ++ Σh2 ++ Σs) ∧
+    Forall2 (λ Σ e, typed Σ ∅ e UnitT) Σs es ∧
+    length Σh1 = length h ∧
+    length Σh2 = length h ∧
+    ∀ l b ct, Σ !! (l,b) = Some ct ->
+      ∃ b1 b2 ct' Σ1 Σ2,
+        Σ !! (l,negb b) = Some ct' ∧
+        lookup_recv h (l,b) = Some b1 ∧
+        lookup_recv h (l,negb b) = Some b2 ∧
+        Σh1 !! l = Some Σ1 ∧
+        Σh2 !! l = Some Σ2 ∧
+        bufs_typed (Σ1, b1, ct) (Σ2, b2, ct').
 
-    Send takes a linear resource from a thread and puts it in one of the buffers of a channel endpoint that
-    the thread owns. This simultaneously steps the session protocol and puts something in the buffer. So this
-    preserves the invariant.
-
-    Receive takes an element out of one of the channel endpoints that the thread owns. This simultaneously steps
-    the session protocol and takes something out of the buffer. So this preserves the invariant.
-*)
-
-Theorem deadlock_freedom e e1 s1 :
-    steps [e] ∅ e1 s1 ->
-    all_values e1 ∨ ∃ e2 s2, step e1 s1 e2 s2.
+Theorem invariant_init e : typed ∅ ∅ e UnitT -> invariant [e] [].
 Proof.
-    intros. induction H.
-    - admit.
-    -
+  intros Ht.
+  unfold invariant.
+  exists ∅, [∅ : heapT], [], []. simpl. split.
+  - exists ∅. unfold disj_union. split; eauto. split.
+    + apply map_disjoint_empty_l.
+    + by rewrite left_id_L.
+  - repeat (split;eauto). intros.
+    by apply lookup_empty_Some in H.
 Qed.
-(*
-    We first check if all threads are values. If so, we return the first disjunct.
-    If there is a thread that's not a value, we will start an iterative process.
-    If the thread is not blocked on receive, we are done, because then the thread can take a step.
-    If it is blocked on receive, we look at which channel it is blocked on, and to which thread
-    the other endpoint is connected to. We continue the iterative process at that thread.
-    Because the connectivity graph is a tree, this process will not go in a cycle, so it eventually
-    terminates at a thread that can take a step.
 
-    The crucial point is that it is never the case that two threads connected to a channel c are
-    both blocked on c. Therefore this iterative process never goes back to where it came from.
-    Instead it follows some path in an acyclic graph, and since the graph is finite this will terminate.
+Lemma disj_union_positive {A B : Type} `{Countable A} (x y : gmap A B) : disj_union ∅ x y -> x = ∅ ∧ y = ∅.
+Proof.
+  unfold disj_union.
+  intros [Hd Hu]. symmetry in Hu. split.
+  - by apply map_positive_l in Hu.
+  - by rewrite map_union_comm in Hu; first apply map_positive_l in Hu.
+Qed.
+
+Lemma disj_union_empty_r {A B : Type} `{Countable A} (x y : gmap A B) : disj_union x y ∅ <-> x = y.
+Proof.
+  unfold disj_union.
+  rewrite right_id; split.
+  - naive_solver.
+  - intros H'. split; auto. apply map_disjoint_empty_r.
+Qed.
+
+Lemma disj_union_sym {A B : Type} `{Countable A} (x y z : gmap A B) : disj_union x y z <-> disj_union x z y.
+Proof.
+  unfold disj_union. split; intros []; split; try (symmetry; done); subst; rewrite map_union_comm; eauto.
+Qed.
+
+Lemma disj_union_singleton_r {A B : Type} `{Countable A} (x : gmap A B) k v k' v' :
+  disj_union {[k := v]} x {[k' := v']} -> x = ∅ ∧ k = k' ∧ v = v'.
+Proof.
+  intros [Hd Hx]. pose proof (f_equal (.!! k') Hx); simplify_map_eq.
+  split; [|done]. apply map_empty; intros k''. apply eq_None_not_Some; intros [y ?].
+  apply (f_equal (.!! k'')) in Hx; simplify_map_eq.
+Qed.
+
+(* Lemma disj_union_singleton_case {A B : Type} `{Countable A} {Γ' Γ Γ1 Γ2 : gmap A B} {x vT} :
+  disj_union Γ' Γ {[x := vT]} ->
+  disj_union Γ' Γ1 Γ2 ->
+  (∃ Γ1', disj_union Γ1 Γ1' {[ x := vT ]}) ∨ (∃ Γ2', disj_union Γ2 Γ2' {[ x:= vT ]}).
+Proof.
+Admitted.
 *)
+
+Lemma disj_union_assoc_l {A B : Type} `{Countable A} {Σ123 Σ23 Σ1 Σ2 Σ3 : gmap A B} :
+  disj_union Σ123 Σ1 Σ23 ->
+  disj_union Σ23 Σ2 Σ3 ->
+  disj_union Σ123 (Σ1 ∪ Σ2) Σ3.
+Proof.
+Admitted.
+
+Lemma disj_union_assoc_r {A B : Type} `{Countable A} {Σ123 Σ23 Σ1 Σ2 Σ3 : gmap A B} :
+  disj_union Σ123 Σ1 Σ23 ->
+  disj_union Σ23 Σ2 Σ3 ->
+  disj_union (Σ1 ∪ Σ2) Σ1 Σ2.
+Proof.
+Admitted.
+
+
+Lemma disj_union_lookup_None_l {A B : Type} `{Countable A} {Γ Γ1 Γ2 : gmap A B} x :
+  disj_union Γ Γ1 Γ2 ->
+  Γ !! x = None ->
+  Γ1 !! x = None.
+Proof.
+  unfold disj_union; intros [? ->] ?. apply lookup_union_None in H1. by destruct H1.
+Qed.
+
+Lemma disj_union_lookup_None_r {A B : Type} `{Countable A} {Γ Γ1 Γ2 : gmap A B} x :
+  disj_union Γ Γ1 Γ2 ->
+  Γ !! x = None ->
+  Γ2 !! x = None.
+Proof.
+  rewrite disj_union_sym. apply disj_union_lookup_None_l.
+Qed.
+
+Lemma typed_no_var_subst Γ Σ e t x v :
+  Γ !! x = None ->
+  typed Σ Γ e t ->
+  subst x v e = e.
+Proof.
+  intros Heq Ht. induction Ht; f_equal/=;
+  eauto using disj_union_lookup_None_l, disj_union_lookup_None_r; case_decide; simplify_map_eq; auto.
+  - f_equal. apply IHHt. destruct H. simplify_map_eq. rewrite lookup_union Heq lookup_singleton_ne; auto.
+  - apply IHHt2. destruct H1. destruct H0. simplify_map_eq. rewrite lookup_union.
+    apply lookup_union_None in Heq. destruct Heq as (_ & ->).
+    rewrite lookup_singleton_ne; auto.
+  - apply IHHt2. destruct H0. destruct H2. simplify_map_eq.
+    rewrite lookup_union. apply lookup_union_None in Heq. destruct Heq as (_ & ->).
+    rewrite lookup_insert_ne; auto. rewrite lookup_singleton_ne; auto.
+Qed.
+
+Lemma disj_union_case {A B : Type} `{Countable A} {Γ Γ0 Γ1 Γ2 : gmap A B} {x v} :
+  disj_union Γ Γ1 Γ2 ->
+  disj_union Γ Γ0 {[x := v]} ->
+  (disj_union Γ1 (delete x Γ1) {[x := v]} ∧ Γ2 !! x = None) ∨
+  (disj_union Γ2 (delete x Γ2) {[x := v]} ∧ Γ1 !! x = None).
+Proof.
+  intros [] []. simplify_map_eq.
+  destruct (Γ1 !! x) eqn:E.
+  - left. split; last eauto using map_disjoint_Some_r.
+    pose proof (f_equal (.!! x) H3). simplify_map_eq. unfold disj_union.
+    rewrite -insert_union_singleton_r; last apply lookup_delete.
+    rewrite insert_delete.
+    rewrite insert_id; auto. split; auto.
+    apply map_disjoint_singleton_r_2.
+    by rewrite lookup_delete.
+  - right. split; auto.
+    pose proof (f_equal (.!! x) H3). simplify_map_eq. unfold disj_union.
+    rewrite -insert_union_singleton_r; last apply lookup_delete.
+    rewrite insert_delete.
+    rewrite insert_id; auto. split; auto.
+    apply map_disjoint_singleton_r_2.
+    by rewrite lookup_delete. apply lookup_union_Some in H1; auto.
+    destruct H1; simplify_eq. auto.
+Qed.
+
+Lemma disj_union_neq {A B : Type} `{Countable A} {Γ Γ' Γ'' : gmap A B} {x1 x2 v1 v2} :
+  disj_union Γ' Γ {[x1 := v1]} ->
+  disj_union Γ'' Γ' {[x2 := v2]} ->
+  x1 ≠ x2 ∧ ∃ Γ2', disj_union Γ2' Γ {[x2 := v2]}.
+Proof.
+  intros [] []. subst. split; first by simplify_map_eq.
+  exists (<[x2 := v2]> Γ).
+  split. solve_map_disjoint. simplify_map_eq. rewrite insert_union_singleton_r; auto.
+Qed.
+
+Lemma subst_typed Σ Σ1 Σ2 Γ Γ1 e eT v vT x :
+  disj_union Σ Σ1 Σ2 ->
+  disj_union Γ Γ1 {[ x := vT ]} ->
+  val_typed Σ1 v vT ->
+  typed Σ2 Γ e eT ->
+  typed Σ Γ1 (subst x v e) eT.
+Proof.
+  intros Ds Dg Hv Ht. revert Ds Dg Hv. revert Γ1 Σ Σ1 x v vT.
+  induction Ht; simpl; intros.
+  - apply disj_union_positive in Dg as [_ Dg]. apply singleton_non_empty in Dg. by exfalso.
+  - apply disj_union_empty_r in Ds. apply disj_union_singleton_r in Dg as (A & B & C). subst.
+    case_decide; first by constructor. by contradict H.
+  - destruct (disj_union_case H0 Dg) as [[]|[]].
+    + erewrite-> (typed_no_var_subst _ _ e2) by done.
+      econstructor; last done.
+      * eapply disj_union_assoc_l; eauto.
+      * admit.
+      * eapply IHHt1.
+       admit. (* map reasoning *)
+    + admit. (* symmetric case *)
+  - destruct (disj_union_neq Dg H) as (Heq & Γ1' & Hdisj). rewrite decide_False; last done.
+    econstructor; eauto. eapply IHHt; eauto.
+    destruct H. destruct Dg. destruct Hdisj. subst.
+    split. solve_map_disjoint. rewrite -assoc_L. rewrite (map_union_comm {[x0 := vT]}). rewrite assoc_L. done. solve_map_disjoint.
+  - admit.
+  - admit.
+  - admit.
+  - admit.
+  - admit.
+  - admit.
+  - constructor. eauto.
+  - constructor. eauto.
+Admitted.
+
+Lemma dual_dual c : dual (dual c) = c.
+Proof.
+  induction c; simpl; auto; rewrite IHc; auto.
+Qed.
+
+Lemma bufs_typed_sym Σ Σ' vs vs' r r' :
+  bufs_typed (Σ,vs,r) (Σ',vs',r') ->
+  bufs_typed (Σ',vs',r') (Σ,vs,r).
+Proof.
+  induction 1.
+  - rewrite<- (dual_dual ct) at 2. constructor.
+  - econstructor; eauto.
+  - econstructor; eauto.
+Qed.
+
+Lemma bufs_typed_sym_iff Σ Σ' vs vs' r r' :
+  bufs_typed (Σ,vs,r) (Σ',vs',r') <->
+  bufs_typed (Σ',vs',r') (Σ,vs,r).
+Proof.
+  split; intros; apply bufs_typed_sym; done.
+Qed.
+
+Lemma unsimpl_dual_recv aT r : RecvT aT (dual r) = dual (SendT aT r).
+Proof. done. Qed.
+
+(*
+Does not hold:
+
+Lemma bufs_typed_recv_l Σ Σ' aT vs r vs' r' :
+  bufs_typed (Σ,vs,RecvT aT r) (Σ',vs',r') ->
+    ∃ Σ1 Σ2 a vs'',
+      vs' = a::vs'' ∧
+      disj_union Σ' Σ1 Σ2 ∧
+      val_typed Σ1 a aT ∧
+      bufs_typed (Σ,vs,r) (Σ2,vs',r').
+Proof.
+  intros H. inversion H; simplify_eq. eauto.
+Qed.
+*)
+
+Lemma bufs_typed_recv_l Σ Σ' a aT vs r vs' r' :
+  bufs_typed (Σ,vs,RecvT aT r) (Σ',a::vs',r') ->
+    ∃ Σ1 Σ2,
+      disj_union Σ' Σ1 Σ2 ∧
+      val_typed Σ1 a aT ∧
+      bufs_typed (Σ,vs,r) (Σ2,vs',r').
+Proof.
+  intros H. inversion H. simplify_eq. eauto.
+Qed.
+
+Lemma bufs_typed_recv_r Σ Σ' a aT vs r vs' r' :
+  bufs_typed (Σ',a::vs',r') (Σ,vs,RecvT aT r) ->
+    ∃ Σ1 Σ2,
+      disj_union Σ' Σ1 Σ2 ∧
+      val_typed Σ1 a aT ∧
+      bufs_typed (Σ2,vs',r') (Σ,vs,r) .
+Proof.
+  intros H. inversion H. simplify_eq. eauto.
+Qed.
+
+Lemma bufs_typed_send_l Σ Σ' Σ1 Σp a aT vs r vs' r' :
+  val_typed Σ1 a aT ->
+  disj_union Σp Σ Σ1 ->
+  bufs_typed (Σ,vs,SendT aT r) (Σ',vs',r') ->
+  bufs_typed (Σp,vs++[a],r) (Σ',vs',r').
+Proof.
+  revert Σ Σ' Σ1 Σp a aT r vs' r'.
+  induction vs as [|v1 vr]; intros Σ Σ' Σ1 Σp a aT r vs' r' Hv Hd Hbt; simpl.
+  - inversion Hbt. simplify_eq.
+    econstructor. 3: econstructor.
+    + apply disj_union_empty_r. apply disj_union_sym in Hd.
+      apply disj_union_empty_r in Hd. eauto.
+    + eauto.
+  - inversion Hbt. simplify_eq.
+    econstructor; last first. 2: done.
+    + eapply IHvr; last done; first done.
+      unfold disj_union in *. split; last done.
+      destruct Hd. destruct H2. simplify_eq.
+      rewrite-> map_disjoint_union_l in H. by destruct H.
+    + unfold disj_union in *.
+      destruct Hd. destruct H2. simplify_eq.
+      split.
+      * rewrite-> map_disjoint_union_l in H. destruct H.
+        symmetry.
+        rewrite map_disjoint_union_l. split; auto.
+      * by rewrite assoc.
+Qed.
+
+Lemma bufs_typed_send_r Σ Σ' Σ1 Σp a aT vs r vs' r' :
+  val_typed Σ1 a aT ->
+  disj_union Σp Σ Σ1 ->
+  bufs_typed (Σ',vs',r') (Σ,vs,SendT aT r) ->
+  bufs_typed (Σ',vs',r') (Σp,vs++[a],r).
+Proof.
+  intros. rewrite-> bufs_typed_sym_iff in H1. rewrite bufs_typed_sym_iff.
+  eapply bufs_typed_send_l; try done.
+Qed.
+
+(*
+Deadlock invariant:
+0. Define the type of abstract states
+
+The abstract state is a graph with threads and channels as vertices.
+We call this graph the connectivity graph.
+
+1. Compute the abstract state for the simple case where all channel endpoints are inside thread exprs
+
+In this case we have an edge from a thread to a channel if the thread has a channel endpoint for that channel.
+
+2. State the invariant that holds for this abstract state.
+
+The (undirected) connectivity graph is acyclic.
+
+3. Generalize to the case where channel endpoints can also appear in the heap
+
+In this case we also have edges between channels and other channels. If we have an endpoint for channel A in a buffer for channel B, then we have an edge from A to B.
+
+4. State the invariant that holds for this abstract state.
+
+Still the same: the (undirected) connectivity graph is acyclic.
+*)
+
+Record connectivity_graph := {
+  thread_outgoing_edges : list (gset loc);
+  channel_outgoing_edges : list (gset loc)
+}.
+
+Fixpoint val_abstract_state (v : val) : gset loc :=
+  match v with
+  | Unit | Nat _ => ∅
+  | Fun _ e => expr_abstract_state e
+  | Pair a b => val_abstract_state a ∪ val_abstract_state b
+  | Chan (l,_) => {[ l ]}
+  end
+with expr_abstract_state (e : expr) : gset loc :=
+  match e with
+  | Val v => val_abstract_state v
+  | Var _ => ∅
+  | Lam _ a | Recv a | Fork a | Close a => expr_abstract_state a
+  | App a b | Send a b | Let _ a b | LetUnit a b | LetProd _ _ a b =>
+    expr_abstract_state a ∪ expr_abstract_state b
+  | If a b c => expr_abstract_state a ∪ expr_abstract_state b ∪ expr_abstract_state c
+  end.
+
+Definition chan_abstract_state (bufs : list val * list val) : gset loc :=
+  let (buf1,buf2) := bufs in
+  union_list ((val_abstract_state <$> buf1) ++ (val_abstract_state <$> buf2)).
+
+Definition compute_abstract_state (es : list expr) (h : heap) : abstract_state :=
+  (expr_abstract_state <$> es, chan_abstract_state <$> h).
+
+
+Definition node := (nat + loc)%type.
+Inductive graph (s : abstract_state) : node -> node -> Prop :=
+  | expr_edge : forall E C i o out,
+    s = (E,C) -> E !! i = Some out -> o ∈ out -> graph s (inl i) (inr o)
+  | chan_edge : forall E C i o out,
+    s = (E,C) -> C !! i = Some out -> o ∈ out -> graph s (inr i) (inr o).
+
+(* Current idea:
+- A simple path is a path without duplicate nodes
+- A tree is a graph where there is a unique simple path between each pair of nodes
+- Can do inductive reasoning because there is a maximum length to simple paths in a finite graph
+*)
+
+(*
+Prior work for deadlocks: type system, language, what kind of proof, how detailed.
+- Honda session types (pi calculus) vs intuitionistic vs classical (vs lambda calculus + channels)
+- Formal vs informal
+- Synchronous vs asynchronous
+- Logic based proof (cut elimination) vs buffer based
+
+Potential publication without separation logic.
+
+Wadler is the most related previous work: he has a linear lambda calculus,
+and "proves" deadlock freedom by translation to pi calculus.
+*)
+
+Theorem invariant_preserved es es' h h' :
+  invariant es h -> step es h es' h' -> invariant es' h'.
+Proof.
+  intros Hinv Hstep.
+  inversion Hstep; simplify_eq.
+  - admit.
+    (* TODO: think about the right induction hypothesis here, for the induction over the context *)
+  - unfold invariant.
+    (* TODO: get the type out of the invariant, then construct the right Σ, and prove the new invariant *)
+    admit.
+Admitted.
+
+Theorem invariant_progress : True.
+Proof.
+Admitted.
