theories/trees.v
@@ -1,0 +1,164 @@
+From iris.proofmode Require Import base tactics classes.
+
+Definition A := nat.
+Definition graph := gset (A * A).
+
+(* 
+We represent a cycle p as a list of nodes. Conceptually, the sequence
+of nodes repeats itself (p..,p..,p..), and represents an infinite
+path in G.
+If p = [x] it represents the cycle [x,x,x,...]. 
+This can only occur if the node x has a self loop in G.
+A cycle is never empty.
+*)
+Definition cycle (p : list A) (G : graph) :=
+  p ≠ [] ∧
+  ∀ i x y,
+    p !! i = Some x ->
+    p !! (S i `mod` length p) = Some y ->
+    (x,y) ∈ G ∨ (y,x) ∈ G.
+
+Lemma baz : cycle [3] (singleton (3,3)).
+Proof.
+  split.
+  - admit.
+  - intros i x y H1 H2.
+    destruct i. simpl in *. simplify_eq.
+    + admit.
+    + simpl in *. admit.
+Qed.
+
+(*
+A cycle has a U-turn if it visits [...,x,y,x,...], that is, 
+it visits x, then y, then goes back to x.
+*)
+Definition has_uturn (p : list A) :=
+  ∃ i x, p !! i = Some x ∧ p !! (i+2 `mod` length p) = Some x.
+
+Definition no_self_loops (G : graph) :=
+  ∀ i, (i,i) ∉ G.
+
+(* Corner cases:
+1. Self loops
+2. Cycles of a single edge and back
+*)
+
+Lemma foo : has_uturn [3;4].
+Proof.
+  exists 0.
+  exists 3.
+  simpl. auto.
+Qed.
+
+Lemma bar : has_uturn [3].
+Proof.
+  exists 0.
+  exists 3.
+  simpl. auto.
+Qed.
+
+Definition tree (G : graph) :=
+  no_self_loops G ∧ (∀ p, cycle p G -> has_uturn p).
+
+Lemma empty_is_tree : tree ∅.
+  split.
+  { intro. apply not_elem_of_empty. } 
+  intros p [Hne Hc].
+  destruct p; simplify_eq.
+  exfalso.
+  destruct p; simplify_eq.
+  - specialize (Hc 0 a a).
+    destruct Hc; eauto.
+    rewrite-> elem_of_empty in H. destruct H.
+    rewrite-> elem_of_empty in H. destruct H.
+  - specialize (Hc 0 a a0).
+    destruct Hc; eauto. simpl.
+    replace (S (length p) - length p) with 1 by lia; done.
+    rewrite-> elem_of_empty in H. destruct H.
+    rewrite-> elem_of_empty in H. destruct H.
+Qed.
+
+Definition lone (x : A) (G : graph) :=
+  ∀ y, (x,y) ∉ G ∧ (y,x) ∉ G.
+
+Lemma cycle_edge_unused G p x y :
+  cycle p (G ∪ {[x, y]}) -> y ∉ p -> cycle p G.
+Proof.
+  intros [Hne Hc] Hnip.
+  split; auto.
+  intros i a b H1 H2.
+  cut ((a, b) ∈ (G ∪ {[x, y]}) ∨ (b, a) ∈ (G ∪ {[x, y]})); last by eauto.
+  assert (a ≠ y) as Ha.
+  { intros H. subst. apply elem_of_list_lookup_2 in H1. done. }
+  assert (b ≠ y) as Hb.
+  { intros H. subst. apply elem_of_list_lookup_2 in H2. done. }
+  rewrite-> !elem_of_union.
+  intros [[]|[]]; auto; exfalso; 
+  rewrite-> elem_of_singleton in H; simplify_eq.
+Qed.
+
+Lemma extend_tree (x y : A) (G : graph) :
+  x ≠ y -> lone y G -> tree G -> tree (G ∪ {[x,y]}).
+Proof.
+  intros Hneq Hl Ht.
+  split.
+  { unfold tree,no_self_loops in *. set_solver. }
+  intros p [Hne Hc].
+  destruct Ht as [Hnocy Huturn].
+  destruct (decide (y ∈ p)).
+  - apply elem_of_list_lookup_1 in e as (i & Hi).
+    exists ((i - 1) `mod` length p).
+    exists x.
+    split.
+    {
+      assert (∃ x0, p !! ((i - 1) `mod` length p) = Some x0).
+      {
+
+      }
+      destruct H.
+      specialize (Hc ((i-1) `mod` length p)).
+      specialize (Hc x0 y).
+      specialize (Hc H).
+      replace ((i - 1) `mod` length p + 1 `mod` length p) with i in Hc by admit.
+      specialize (Hc Hi).
+      destruct (Hl x0) as [Hlx0 Hl0x].
+      destruct Hc.
+      {
+        rewrite-> elem_of_union in H0.
+        destruct H0.
+        - exfalso. by apply Hl0x.
+        - apply elem_of_singleton in H0. simplify_eq. done.
+      }
+      { 
+        rewrite-> elem_of_union in H0.
+        destruct H0.
+        - exfalso. by apply Hlx0.
+        - apply elem_of_singleton in H0. simplify_eq.
+      }
+    }
+    replace ((i - 1) `mod` strings.length p + 2 `mod` strings.length p) 
+      with ((i + 1) `mod` strings.length p) by admit.
+    {
+
+    }
+  - apply Huturn. by eapply cycle_edge_unused.
+Admitted.
+
+Lemma modify_tree (x y z : A) (G : graph) :
+  (x,y) ∈ G -> (y,z) ∉ G ->
+  tree (G ∪ {[y,z]}) -> 
+  tree (G ∪ {[x,z]}).
+Proof.
+Admitted.
+
+Definition cardinality_at_most (n : nat) (G : graph) :=
+  ∃ V : list A,
+    length V = n ∧
+    ∀ x y, (x,y) ∈ G -> x ∈ V ∧ y ∈ V.
+
+Lemma long_paths_have_uturns (G : graph) (p : list A) (n : nat) :
+  cardinality_at_most n G ->
+  tree G -> path p G -> 
+  length p > n -> has_uturn p.
+Proof.
+Admitted.
