theories/trees3.v
@@ -1,0 +1,542 @@
+From stdpp Require Import gmap.
+From stdpp Require Import base.
+
+Definition lookup_mod `{Inhabited A} (i : Z) (xs : list A) : A :=
+  xs !!! (Z.to_nat (i `mod` length xs)).
+
+Lemma lookup_mod_mod `{Inhabited A} (xs : list A) (i : Z) :
+  lookup_mod i xs = lookup_mod (i + length xs) xs.
+Proof.
+  intros.
+  unfold lookup_mod.
+  f_equiv. f_equiv.
+  rewrite Zplus_mod, Z_mod_same_full, Z.add_0_r, Zmod_mod. done.
+Qed.
+
+Lemma lookup_mod_some {A} (xs : list A) (i : Z) :
+  length xs ≠ 0 -> is_Some (xs !! Z.to_nat (i `mod` length xs)).
+Proof.
+  intro.
+  apply lookup_lt_is_Some_2.
+  pose proof (Z_mod_lt i (length xs)) as []. lia. lia.
+Qed.
+
+Lemma elem_of_list_lookup_mod `{Inhabited A} (xs : list A) (x : A) :
+  x ∈ xs -> ∃ (i : Z), lookup_mod i xs = x.
+Proof.
+  intros Hin.
+  apply elem_of_list_lookup_1 in Hin as [i Hi].
+  exists i. unfold lookup_mod.
+  apply list_lookup_total_correct.
+  rewrite Zmod_small,Nat2Z.id; auto.
+  split; [lia|].
+  apply lookup_lt_Some in Hi. lia.
+Qed.
+
+Lemma elem_of_list_lookup_mod_r `{Inhabited A} (xs : list A) (x : A) (i : Z) :
+  length xs ≠ 0 -> lookup_mod i xs = x -> x ∈ xs.
+Proof.
+  intros Hlen Hlookup.
+  eapply elem_of_list_lookup_2.
+  unfold lookup_mod in *.
+  rewrite list_lookup_total_alt in Hlookup.
+  pose proof (lookup_mod_some xs i Hlen) as [].
+  rewrite H0 in Hlookup. simpl in *. simplify_eq. eauto.
+Qed.
+
+Lemma NoDup_lookup_mod `{Inhabited A} (xs : list A) (i j : Z) (x : A) :
+  NoDup xs → lookup_mod i xs = lookup_mod j xs ->
+  ((i - j) `mod` length xs = 0)%Z.
+Proof.
+  unfold lookup_mod.
+  rewrite !list_lookup_total_alt.
+  destruct (decide (length xs = 0)) as [Hzero|?].
+  { rewrite Hzero. rewrite !Zmod_0_r. simpl. reflexivity. }
+  destruct (lookup_mod_some xs i) as [y E]; [done|].
+  destruct (lookup_mod_some xs j) as [z F]; [done|].
+  rewrite E, F. simpl.
+  intros Hnodup ->.
+  pose proof (NoDup_lookup xs _ _ z Hnodup E F) as Heq.
+  apply Z2Nat.inj in Heq; eauto using Z_mod_pos with lia.
+  rewrite Zminus_mod, Heq, Z.sub_diag. reflexivity.
+Qed.
+
+Lemma uturn_has_dup `{Inhabited A} (xs : list A) (i : Z) :
+  NoDup xs -> length xs >= 3 -> lookup_mod (i-1)%Z xs = lookup_mod (i+1)%Z xs -> False.
+Proof.
+  intros Hnodup Hlen Heq.
+  symmetry in Heq.
+  apply NoDup_lookup_mod in Heq; [|exact inhabitant|done].
+  replace (i + 1 - (i - 1))%Z with 2%Z in Heq by lia.
+  rewrite Zmod_small in Heq;[discriminate|lia].
+Qed.
+
+Definition graph A `{Countable A} := gset (A * A).
+
+Section graph.
+  Context `{Countable A}.
+  Context `{Inhabited A}.
+  Definition undirected (g : graph A) :=
+    ∀ x y, (x,y) ∈ g → (y,x) ∈ g.
+  Definition no_self_loops (g : graph A) :=
+    ∀ x, (x,x) ∉ g.
+  Definition lookup_edge (i : Z) (xs : list A) :=
+    (lookup_mod i xs, lookup_mod (i+1) xs).
+  Record cycle (g : graph A) (xs : list A) : Prop := Cycle {
+    cycle_length : 3 <= length xs;
+    cycle_NoDup : NoDup xs;
+    cycle_cycle : ∀ i, lookup_edge i xs ∈ g;
+  }.
+  Record tree (g : graph A) : Prop := Tree {
+    tree_undirected : undirected g;
+    tree_no_self_loops : no_self_loops g;
+    tree_no_cycle xs : ¬cycle g xs;
+  }.
+  Lemma undirected_empty : undirected ∅.
+  Proof. unfold undirected. set_solver. Qed.
+  Lemma no_self_loops_empty : no_self_loops ∅.
+  Proof. unfold no_self_loops. set_solver. Qed.
+  Lemma no_cycle_empty xs : ¬cycle ∅ xs.
+  Proof.
+    destruct 1 as [Hlen _ Hcycle].
+    destruct xs as [|x1 [|x2 xs]]; simplify_eq/=; [lia..|].
+    specialize (Hcycle 0). set_solver.
+  Qed.
+  Lemma tree_empty : tree ∅.
+  Proof.
+    split; eauto using undirected_empty, no_self_loops_empty, no_cycle_empty.
+  Qed.
+  Definition lone (x : A) (g : graph A) :=
+    ∀ y, (x,y) ∉ g.
+  Definition graph_singleton (x y : A) : graph A := {[ (x,y); (y,x) ]}.
+  Lemma graph_singleton_elem (x y a b : A) :
+    (a,b) ∈ graph_singleton x y <-> (a = x ∧ b = y) ∨ (a = y) ∧ (b = x).
+  Proof. unfold graph_singleton. set_solver. Qed.
+  Lemma graph_singleton_sym (x y : A) : 
+    graph_singleton x y = graph_singleton y x.
+  Proof. unfold graph_singleton. set_solver. Qed.
+  Lemma graph_singleton_elem_1 (x y z : A) :
+    (y,z) ∈ graph_singleton x y → z = x.
+  Proof. unfold graph_singleton. set_solver. Qed.
+  Lemma graph_singleton_elem_2 (x y z : A) :
+    (z,y) ∈ graph_singleton x y → z = x.
+  Proof. unfold graph_singleton. set_solver. Qed.
+  Lemma undirected_extend (x y : A) (g : graph A) :
+    undirected g → undirected (g ∪ graph_singleton x y).
+  Proof. unfold undirected, graph_singleton. set_solver. Qed.
+  Lemma no_self_loops_extend (x y : A) (g : graph A) :
+    x ≠ y →
+    no_self_loops g → no_self_loops (g ∪ graph_singleton x y).
+  Proof. unfold no_self_loops, graph_singleton. set_solver. Qed.
+  Lemma cycle_extend (x y : A) (g : graph A) xs :
+    undirected g →
+    x ≠ y → lone y g →
+    cycle (g ∪ graph_singleton x y) xs →
+    cycle g xs.
+  Proof.
+    intros Hundir Hneq Hlone [Hlen Hnodup Hcycle].
+    assert (y ∉ xs).
+    {
+      intro Hin.
+      apply elem_of_list_lookup_mod in Hin as [i Helem].
+      unfold lookup_edge in *.
+      assert (lookup_mod (i+1) xs = x).
+      {
+        specialize (Hcycle i).
+        apply elem_of_union in Hcycle as [].
+        - specialize (Hlone (lookup_mod (i+1) xs)). set_solver.
+        - rewrite-> Helem in *. eapply graph_singleton_elem_1; done.
+      }
+      assert (lookup_mod (i-1) xs = x).
+      {
+        specialize (Hcycle (i-1)%Z).
+        replace (i - 1 + 1)%Z with i in * by lia.
+        apply elem_of_union in Hcycle as [].
+        - specialize (Hlone (lookup_mod (i-1) xs)).
+          unfold undirected in *.  set_solver.
+        - rewrite-> Helem in *. eapply graph_singleton_elem_2; done.
+      }
+      subst. eapply uturn_has_dup; (done || lia).
+    }
+    split; [by auto..|].
+    intros i.
+    specialize (Hcycle i).
+    apply elem_of_union in Hcycle as []; auto.
+    unfold graph_singleton in *.
+    unfold lookup_edge in *.
+    set_solver by eauto using elem_of_list_lookup_mod_r with lia.
+  Qed.
+  
+  Lemma tree_extend (x y : A) (g : graph A) :
+    x ≠ y → lone y g →
+    tree g → tree (g ∪ graph_singleton x y).
+  Proof.
+    intros ?? [].
+    split; eauto using undirected_extend, no_self_loops_extend.
+    intros ??. specialize (tree_no_cycle0 xs). apply tree_no_cycle0.
+    eapply cycle_extend; eauto.
+  Qed.
+
+  Lemma undirected_delete (x y : A) (g : graph A) :
+    undirected g ->
+    undirected (g ∖ graph_singleton x y).
+  Proof.
+    intros Hundir a b.
+    rewrite !elem_of_difference.
+    intros [].
+    split.
+    - by apply Hundir.
+    - unfold graph_singleton in *. set_solver.
+  Qed.
+
+  Lemma no_self_loops_delete (x y : A) (g : graph A) :
+    x ≠ y -> no_self_loops g ->
+    no_self_loops (g ∖ graph_singleton x y).
+  Proof.
+    intros Hneq Hsl a [H1 ?]%elem_of_difference.
+    apply Hsl in H1 as [].
+  Qed.
+
+  Lemma dec_exists_list {B} (xs : list B) (P : B → Prop) :
+  (∀ x, P x → x ∈ xs) → (∀ x, x ∈ xs → Decision (P x)) → Decision (∃ x, P x).
+  Proof.
+    intros HPxs Hdec.
+    induction xs as [|x xs IHxs]. { right. set_solver. }
+    assert (Decision (P x)) as [] by (apply Hdec; set_solver).
+    { left. naive_solver. }
+    apply IHxs.
+    - intros x' HPx'. specialize (HPxs x' HPx').
+      assert (x' = x ∨ x' ∈ xs) as []; set_solver.
+    - intros ??. apply Hdec. set_solver.
+  Qed.
+
+  Lemma exists_lookup_mod_dec (n : nat) (P : nat -> Prop) :
+    (∀ i, Decision (P i)) ->
+    Decision (∃ i, P i ∧ i < n).
+  Proof.
+    intros Hdec.
+    eapply (dec_exists_list (seq 0 n)).
+    - intros ? []. rewrite elem_of_list_In. apply in_seq. lia.
+    - solve_decision.
+  Qed.
+
+  Lemma lookup_reverse {B} (i : nat) (xs : list B) :
+    i < length xs -> rev xs !! i = xs !! (length xs - S i).
+  Proof.
+    revert i; induction xs; intros; simpl; eauto.
+    assert (length (rev xs) = length xs) by eauto using rev_length.
+    destruct (decide (i = length xs)).
+    {
+      rewrite lookup_app_r; try lia. simplify_eq. rewrite H2.
+      replace (length xs - length xs) with 0 by lia.
+      done.
+    }
+    rewrite lookup_app_l;[|simpl in *;rewrite H2;lia].
+    replace (a :: xs) with ([a] ++ xs) by done.
+    rewrite lookup_app_r; simpl; try lia.
+    rewrite IHxs.
+    f_equiv. lia. simpl in *. lia. simpl in *. lia.
+  Qed.
+
+  Lemma NoDup_rev {B} (xs : list B) :
+    NoDup xs -> NoDup (rev xs).
+  Proof.
+    rewrite !NoDup_alt.
+    intros.
+    assert (i < length xs). { rewrite <-rev_length. by eapply lookup_lt_Some. }
+    assert (j < length xs). { rewrite <-rev_length. by eapply lookup_lt_Some. }
+    rewrite lookup_reverse in H2; eauto.
+    rewrite lookup_reverse in H3; eauto.
+    assert (length xs - S i = length xs - S j). eauto.
+    lia.
+  Qed.
+
+  Lemma lookup_mod_rev (i : Z) (xs : list A) :
+    lookup_mod i xs = lookup_mod (- i - 1) (rev xs).
+  Proof.
+    destruct (decide (length xs = 0)).
+    {
+      destruct xs; simpl in *; simplify_eq.
+      unfold lookup_mod.
+      rewrite !list_lookup_total_alt, !lookup_nil. done.
+    }
+    unfold lookup_mod.
+    rewrite rev_length.
+    rewrite !list_lookup_total_alt.
+    rewrite lookup_reverse.
+    {
+      subst. rewrite<- !list_lookup_total_alt. f_equiv.
+      revert n.
+      generalize (length xs). intros.
+      rewrite<- Z2Nat.inj_succ;[|apply Z_mod_pos; lia].
+      replace n with (Z.to_nat (Z.of_nat n));[|lia].
+      rewrite<- Z2Nat.inj_sub.
+      2: {
+        assert (0 <= (- i - 1) `mod` Z.to_nat n)%Z.
+        apply Z_mod_pos. lia. lia.
+      }
+      f_equiv.
+      assert (n = 37) by admit.
+      assert (i = 163) by admit.
+      subst. done.
+    }
+    destruct (Z.mod_pos_bound (- i - 1) (length xs)). lia. lia.
+  Admitted.
+
+  Lemma cycle_rev (g : graph A) (xs : list A) :
+    undirected g ->
+    cycle g xs -> cycle g (rev xs).
+  Proof.
+    intros Hundir [].
+    constructor.
+    - rewrite rev_length. lia.
+    - apply NoDup_rev. done.
+    - intros i.
+      unfold lookup_edge in *.
+(*       
+      rewrite<- lookup_mod_rev.
+      replace (- (i + 1) - 1)%Z with (- i - 2)%Z by lia.
+      replace (-i - 1)%Z with ((-i - 2)+1)%Z by lia.
+      apply Hundir.
+      apply cycle_cycle0.
+  Qed. *)
+
+  Lemma cycle_mono (g h : graph A) (xs : list A) :
+    cycle g xs -> cycle (g ∪ h) xs.
+  Proof.
+    intros []. constructor; eauto.
+    intro. apply elem_of_union_l. done.
+  Qed.
+
+  Lemma cycle_mono' (g h : graph A) (xs : list A) :
+    cycle (g ∖ h) xs -> cycle g xs.
+  Proof.
+    intros []. constructor; eauto.
+    intro. eapply elem_of_difference. done.
+  Qed.
+
+  Lemma cycle_edge_unused (g : graph A) (x y : A) (xs : list A) :
+    cycle (g ∪ graph_singleton x y) xs ->
+    (∀ i, lookup_edge i xs = (x,y) ∨ lookup_edge i xs = (y,x) -> False) ->
+    cycle g xs.
+  Proof.
+    intros [] Hi. constructor; eauto.
+    intro. specialize (cycle_cycle0 i).
+    rewrite elem_of_union in cycle_cycle0.
+    destruct cycle_cycle0. done.
+    exfalso. apply (Hi i).
+    unfold lookup_edge in *.
+    rewrite graph_singleton_elem in *.
+    naive_solver.
+  Qed.
+
+  Definition delete_mod (i : Z) (xs : list A) : list A.
+  Admitted.
+  
+  Definition insert_mod (i : Z) (x : A) (xs : list A) : list A.
+  Admitted.
+
+  Lemma insert_mod_length (i : Z) (x : A) (xs : list A) :
+    length (insert_mod i x xs) = 1 + length xs.
+  Proof. Admitted.
+
+  Lemma delete_mod_length (i : Z) (xs : list A) :
+    length (delete_mod i xs) = length xs - 1.
+  Proof. Admitted.
+
+  Lemma insert_mod_NoDup (i : Z) (x : A) (xs : list A) :
+    x ∉ xs -> NoDup xs -> NoDup (insert_mod i x xs).
+  Proof. Admitted.
+
+  Lemma delete_mod_NoDup (i : Z) (xs : list A) :
+    NoDup xs -> NoDup (delete_mod i xs).
+  Proof. Admitted.
+
+  Definition edges (xs : list A) : gset (A * A). Admitted.
+
+  Lemma edges_delete (xs : list A) (a b c : A) (i : nat) :
+    3 ≤ length xs ->
+    lookup_mod i xs = a ->
+    lookup_mod (i+1) xs = b ->
+    lookup_mod (i+2) xs = c ->
+    edges (delete_mod (i+1) xs) = edges xs ∖ {[a,b]} ∖ {[b,c]} ∪ {[a,c]}.
+  Proof. Admitted.
+
+  Lemma edges_insert (xs : list A) (a b c : A) (i : nat) :
+    3 ≤ length xs ->
+    lookup_mod i xs = a ->
+    lookup_mod (i+1) xs = c ->
+    edges (insert_mod (i+1) b xs) = edges xs ∖ {[a,c]} ∪ {[a,b]} ∪ {[b,c]}.
+  Proof. Admitted.
+
+  Lemma lookup_edge_mod (i : Z) (xs : list A) :
+    length xs ≠ 0 ->
+    lookup_edge (i `mod` length xs) xs = lookup_edge i xs.
+  Proof.
+    intro.
+    unfold lookup_edge.
+    unfold lookup_mod.
+    rewrite Z.add_mod_idemp_l; [|lia].
+    rewrite Zmod_mod. done.
+  Qed.
+
+  Lemma lookup_mod_rev_2 (i : Z) (xs : list A) :
+    lookup_mod i (rev xs) = lookup_mod (- i - 1) xs.
+  Proof.
+    replace (lookup_mod (- i - 1) xs) with (lookup_mod (- i - 1) (rev (rev xs))).
+    - rewrite lookup_mod_rev. done.
+    - f_equiv. rewrite rev_involutive. done.
+  Qed.
+
+  Definition swap {A} (p : A * A) := 
+      let (a,b) := p in (b,a).
+
+  Lemma lookup_edge_reverse (i : Z) (xs : list A) :
+    lookup_edge (- i - 2) (rev xs) = swap (lookup_edge i xs).
+  Proof.
+    unfold lookup_edge. unfold swap.
+    rewrite !lookup_mod_rev_2. f_equiv.
+    f_equiv. lia. f_equiv. lia.
+  Qed.
+
+  Lemma no_cycle_modify (x y z : A) (xs : list A) (g : graph A) :
+    x ≠ z -> y ≠ z ->
+    tree g -> (x,y) ∈ g -> (x,z) ∈ g ->
+    ¬ cycle (g ∖ graph_singleton x z ∪ graph_singleton y z) xs.
+  Proof.
+    intros Hxneqz Hyneqz [] Hxyg Hxzg Hcycle.
+    assert (Decision (∃ i, 
+      lookup_edge i xs = (y,z) ∨ 
+      lookup_edge i xs = (z,y))).
+    {
+      assert (Decision (∃ i,
+        0 <= i ∧ i < length xs ∧ 
+        (lookup_edge i xs = (y,z) ∨ 
+        lookup_edge i xs = (z,y))))%Z.
+      {
+        apply (dec_exists_list (map Z.of_nat (seq 0 (length xs))))%Z.
+        {
+          intros. rewrite elem_of_list_In, in_map_iff.
+          exists (Z.to_nat x0). split. lia.
+          rewrite in_seq. lia.
+        }
+        solve_decision.
+      }
+      destruct H1.
+      - left. destruct e. exists x0. naive_solver.
+      - right. intro. destruct H1. apply n.
+        exists (x0 `mod` (length xs))%Z.
+        pose proof (Z.mod_pos_bound x0 (length xs)).
+        destruct Hcycle.
+        split. lia.
+        split. lia.
+        rewrite lookup_edge_mod;[|lia].
+        done.
+    }
+    
+    destruct H1 as [Hedge|Hnotedge].
+    2: {
+      apply (tree_no_cycle0 xs).
+      eapply cycle_mono'.
+      eapply cycle_edge_unused. done.
+      naive_solver.
+    }
+    destruct Hedge as [i Hedge].
+    revert i Hedge Hcycle Hxzg Hxyg tree_no_cycle0 tree_no_self_loops0
+            tree_undirected0 Hxneqz Hyneqz.
+    revert xs x y z.
+    cut (∀ (xs : list A) (x y z : A) (i : Z),
+      lookup_edge i xs = (z, y)
+      → cycle (g ∖ graph_singleton x z ∪ graph_singleton y z) xs
+        → (x, z) ∈ g
+          → (x, y) ∈ g
+            → (∀ xs0 : list A, ¬ cycle g xs0)
+              → no_self_loops g → undirected g → x ≠ z → y ≠ z → False).
+    {
+      intros.
+      destruct Hedge; eauto.
+      specialize (H1 (rev xs)).
+      specialize (H1 x y z).
+      eapply H1; eauto. rewrite lookup_edge_reverse.
+      simpl. unfold lookup_edge in H2. simplify_eq. done.
+      apply cycle_rev; eauto.
+      apply undirected_extend.
+      apply undirected_delete. 
+      done.
+    }
+    intros xs x y z.
+    intros i Hedge Hcycle Hxzg Hxyg tree_no_cycle0 tree_no_self_loops0
+            tree_undirected0 Hxneqz Hyneqz.
+    destruct Hcycle.
+
+    destruct (decide (lookup_mod (i+2) xs = x)) as [Hx|Hnx].
+    - apply (tree_no_cycle0 (delete_mod (i+1) xs)).
+      constructor.
+      + (* prove that the length wasn't 3 *)
+        destruct (decide (length xs = 3)); [|rewrite delete_mod_length;lia].
+        exfalso.
+        specialize (cycle_cycle0 (i+2)%Z).
+        assert (lookup_edge (i+2)%Z xs = (x,z)).
+        {
+          unfold lookup_edge in *.
+          replace (i + 2 + 1)%Z with (i + length xs)%Z by lia.
+          rewrite<- lookup_mod_mod. simplify_eq. done.
+        }
+        rewrite H1 in cycle_cycle0.
+        rewrite elem_of_union in cycle_cycle0.
+        rewrite elem_of_difference in cycle_cycle0.
+        destruct cycle_cycle0 as [[]|].
+        * rewrite graph_singleton_elem in *. naive_solver.
+        * rewrite graph_singleton_elem in *.
+          assert (x = y). naive_solver.
+          eapply tree_no_self_loops0. subst. eauto.
+      + apply delete_mod_NoDup. done.
+      + intros j.
+        admit.
+    - apply (tree_no_cycle0 (insert_mod (i+1) x xs)).
+      constructor.
+      + rewrite insert_mod_length. lia.
+      + apply insert_mod_NoDup; [|done]. intro.
+        (* if x is in xs, we can construct a smaller cycle *)
+        
+        admit.
+      + intros j.
+        (* prove that after inserting x, the cycle is in g *)
+        admit.
+  Admitted.
+
+  Lemma tree_modify (x y z : A) (g : graph A) :
+    x ≠ z -> y ≠ z ->
+    tree g -> (x,y) ∈ g -> (x,z) ∈ g ->
+    tree ((g ∖ graph_singleton x z) ∪ graph_singleton y z).
+  Proof.
+    intros ?? [] ??.
+    constructor.
+    - apply undirected_extend. apply undirected_delete. done.
+    - apply no_self_loops_extend;[done|]. 
+      apply no_self_loops_delete;done.
+    - intros. eapply no_cycle_modify; done. 
+  Qed.
+
+  Lemma tree_delete (x y : A) (g : graph A) :
+    tree g -> tree (g ∖ graph_singleton x y).
+  Proof.
+
+  Admitted.
+
+  Definition cardinality_at_most (n : nat) (g : graph A) :=
+    ∃ V : list A,
+      length V = n ∧
+      ∀ x y, (x,y) ∈ g -> x ∈ V ∧ y ∈ V.
+
+  Definition no_u_turn (xs : list A) :=
+    ∀ i x y, xs !! i = Some x -> xs !! (i+2) = Some y -> x ≠ y.
+
+  Lemma no_u_turn_tree_paths_are_short (g : graph A) (xs : list A) (n : nat) :
+    cardinality_at_most n g ->
+    tree g -> path g xs -> no_u_turn xs ->
+    length xs <= n.
+  Proof.
+  Admitted.
+  
+  (* set_wf *)
